theories/Syntax/StrictPos.v
@@ -22,8 +22,14 @@ Set Default Proof Using "Type".
 
 Record ind_sig : Type := {
   Shape : Type;
+  (* Number of non-recursive constructor parameters (finitary). *)
+  param_arity : Shape -> nat;
+  (* Number of recursive constructor fields (finitary). *)
   arity : Shape -> nat;
 }.
+
+Definition ParamPos (Σ : ind_sig) (s : Shape Σ) : Type :=
+  Fin.t (param_arity Σ s).
 
 Definition Pos (Σ : ind_sig) (s : Shape Σ) : Type :=
   Fin.t (arity Σ s).
@@ -34,22 +40,35 @@ Inductive ind_carrier (Σ : ind_sig) : Type :=
 Arguments sup {_} _ _.
 
 Definition ind_zero : ind_sig :=
-  {| Shape := Empty_set; arity := fun e => match e with end |}.
+  {| Shape := Empty_set
+   ; param_arity := fun e => match e with end
+   ; arity := fun e => match e with end |}.
 
 Definition ind_const (A : Type) : ind_sig :=
-  {| Shape := A; arity := fun _ => 0 |}.
+  {| Shape := A
+   ; param_arity := fun _ => 0
+   ; arity := fun _ => 0 |}.
 
 Definition ind_sum (Σ1 Σ2 : ind_sig) : ind_sig :=
-  {| Shape := (Shape Σ1 + Shape Σ2)%type;
-     arity := fun s =>
+  {| Shape := (Shape Σ1 + Shape Σ2)%type
+   ; param_arity := fun s =>
+       match s with
+       | inl s1 => param_arity Σ1 s1
+       | inr s2 => param_arity Σ2 s2
+       end
+   ; arity := fun s =>
        match s with
        | inl s1 => arity Σ1 s1
        | inr s2 => arity Σ2 s2
        end |}.
 
 Definition ind_prod (Σ1 Σ2 : ind_sig) : ind_sig :=
-  {| Shape := (Shape Σ1 * Shape Σ2)%type;
-     arity := fun s =>
+  {| Shape := (Shape Σ1 * Shape Σ2)%type
+   ; param_arity := fun s =>
+       match s with
+       | (s1, s2) => param_arity Σ1 s1 + param_arity Σ2 s2
+       end
+   ; arity := fun s =>
        match s with
        | (s1, s2) => arity Σ1 s1 + arity Σ2 s2
        end |}.
